refactor: eliminate vs_storage/vs_transient denormalization, fix merge_callee_state
State model:
- Remove vs_storage field; sload/sstore go through vs_accounts via contract_storage
- Change vs_transient from storage to transient_storage (address -> storage)
- Add contract_storage, contract_transient accessors

External call semantics:
- merge_callee_state: propagate logs, immutables, allocas; revert-safe storage
- extract_venom_result: simplified (no storage/transient branching)
- Fix external call reentrancy: storage changes visible through vs_accounts

Downstream proof updates:
- stateEquiv, execEquiv, simulation framework adapted to new fields
- write_effects_sound_balance -> write_effects_sound_accounts

venom/simulation/defs/execEquivParamDefsScript.sml
@@ -37,7 +37,6 @@ Definition valid_state_rel_def:
       s1.vs_block_ctx = s2.vs_block_ctx /\
       s1.vs_accounts = s2.vs_accounts /\
       s1.vs_memory = s2.vs_memory /\
-      s1.vs_storage = s2.vs_storage /\
       s1.vs_transient = s2.vs_transient /\
       s1.vs_returndata = s2.vs_returndata /\
       s1.vs_halted = s2.vs_halted /\
@@ -59,7 +58,6 @@ Definition valid_state_rel_def:
       s1.vs_block_ctx = s2.vs_block_ctx /\
       s1.vs_accounts = s2.vs_accounts /\
       s1.vs_memory = s2.vs_memory /\
-      s1.vs_storage = s2.vs_storage /\
       s1.vs_transient = s2.vs_transient /\
       s1.vs_returndata = s2.vs_returndata /\
       s1.vs_halted = s2.vs_halted /\
@@ -99,7 +97,6 @@ Definition valid_state_rel_def:
       t1.vs_block_ctx = t2.vs_block_ctx /\
       t1.vs_accounts = t2.vs_accounts /\
       t1.vs_memory = t2.vs_memory /\
-      t1.vs_storage = t2.vs_storage /\
       t1.vs_transient = t2.vs_transient /\
       t1.vs_returndata = t2.vs_returndata /\
       t1.vs_halted = t2.vs_halted /\
@@ -123,7 +120,6 @@ Definition valid_state_rel_def:
       t1.vs_block_ctx = t2.vs_block_ctx /\
       t1.vs_accounts = t2.vs_accounts /\
       t1.vs_memory = t2.vs_memory /\
-      t1.vs_storage = t2.vs_storage /\
       t1.vs_transient = t2.vs_transient /\
       t1.vs_returndata = t2.vs_returndata /\
       t1.vs_halted = t2.vs_halted /\
