venom/simulation/proofs/execEquivParamHelpersScript.sml
@@ -35,7 +35,7 @@ Theorem vsr_step_inst_pure2:
   !R_ok R_term inst s1 s2.
     valid_state_rel R_ok R_term /\ R_ok s1 s2 /\
     MEM inst.inst_opcode [ADD;SUB;MUL;Div;SDIV;Mod;SMOD;Exp;
-      AND;OR;XOR;SHL;SHR;SAR;SIGNEXTEND;EQ;LT;GT;SLT;SGT;GEP] /\
+      AND;OR;XOR;SHL;SHR;SAR;SIGNEXTEND;BYTE;EQ;LT;GT;SLT;SGT;GEP] /\
     (!x. MEM (Var x) inst.inst_operands ==> lookup_var x s1 = lookup_var x s2) ==>
     lift_result R_ok R_term (step_inst_base inst s1) (step_inst_base inst s2)
 Proof
